EHoare_Triple.v
@@ -1,95 +1,141 @@
-From Rela Require Import EBexp.
+From Rela Require Import EVcg.
+
+Locate set.
+
 From Rela Require Import ECom.
-From Rela Require Import Sigma.
+From Rela Require Import Bexp.
 From Rela Require Import Lambda.
-From Rela Require Import Vcg.
 From Rela Require Import Label.
+From Rela Require Import Sigma.
 
-Definition ceval_f_i_p (s : sigma) (la: lambda) (ps: Psi.psi) (p : prog) (Q : lambda -> Prop) := 
-  forall i,
-  match ceval_prog s la ps p i with
-  | None => True
-  | Some (s') => Q (Post |-> s' ; (Pre |-> s ; la ))
-  end.
+From Coq Require Import Bool.Bool.
+From Coq Require Import Init.Nat.
+From Coq Require Import Arith.Arith.
+From Coq Require Import Arith.EqNat.
 
-Definition hoare_triple_p (P Q: lambda -> Prop) (p : prog) (la: lambda) (ps : Psi.psi) : Prop :=
-  forall s,  P (Pre |-> s ; la ) ->  ceval_f_i_p s la ps p Q .
+Definition hoare_triple_c (P Q: assertion) (c : com) (l: Label.t) (ps : Psi.psi) : Prop :=
+  forall s la s',  P s la -> ceval_c c s la l ps s' -> Q s' (l |-> s ; la ).
 
-Definition ceval_f_i_c (s : sigma) (la: lambda) (l: Label.t) (ps: Psi.psi) (c : com) (Q : lambda -> Prop) := 
-  forall i,
-  match ceval_com s l la ps c i with
-  | None => True
-  | Some (s') => Q (Post |-> s' ; (Pre |-> s ; la ))
-  end.
+Definition hoare_triple_p (P Q: assertion) (p : prog) (ps : Psi.psi) : Prop :=
+  forall s la s' la',  P s la -> ceval_p p s la ps s' la' -> Q s' la'.
 
-Definition hoare_triple_c (P Q: lambda -> Prop) (c : com) (l: Label.t) (la: lambda) (ps : Psi.psi) : Prop :=
-  forall s,  P (Pre |-> s ; la ) ->  ceval_f_i_c s la l ps c Q.
+Definition clause_p (P Q: assertion) (p : prog) (l: Label.t) (ps : Psi.psi) : Prop :=
+  forall s la s' la',  P s la -> ceval_p p s (l |-> s ; la ) ps s' la' -> Q s' (l |-> s ; la ).
+  
+  (*clause et hoare ne sont pas compatible*)
 
-Fixpoint well_c (c : com) : Prop :=
+Lemma seq_hoare_triple :
+forall c l p ps (P Q R: assertion),
+hoare_triple_c P R c l ps ->
+hoare_triple_p R Q p ps ->
+hoare_triple_p P Q (pconst l c p) ps.
+Proof.
+unfold hoare_triple_c.
+unfold hoare_triple_p.
+intros c l p ps P Q R H1 H2 s la s' la' Pre H12. inversion H12; subst.
+eapply H2. eapply H1. apply Pre. apply H9. apply H10.
+Qed.
+
+Definition bassn b :=
+  fun st => (beval st b = true).
+
+Lemma bexp_eval_true : forall b st,
+  beval st b = true -> (bassn b) st.
+Proof. auto. Qed.
+
+Lemma bexp_eval_false : forall b st,
+  beval st b = false ->  ~((bassn b) st).
+Proof. congruence. Qed.
+
+Lemma if_hoare_triple :
+forall p1 p2 l b ps (P Q: assertion),
+clause_p (fun s la => P s la /\ beval s b = true) Q p1 l ps ->
+clause_p (fun s la => P s la /\ beval s b = false) Q p2 l ps ->
+hoare_triple_c P Q (CIf b p1 p2) l ps.
+Proof.
+intros p1 p2 l b ps P Q HTrue HFalse s la s' HP HE.
+inversion HE;subst. 
+- unfold clause_p in HTrue.
+  eapply HTrue.
+  + split. 
+      * apply HP. 
+      * assumption.
+  + apply H8.
+- unfold clause_p in HFalse.
+  eapply HFalse.
+  + split. 
+      * apply HP. 
+      * assumption.
+  + apply H8.
+Qed.
+
+Definition well_c (c : com) : Prop :=
 match c with
 | CSkip => True
 | _ => False
-end
-with well_p (p : prog) : Prop :=
+end.
+
+Fixpoint well_p (p : prog) : Prop :=
 match p with 
 | pnil => True
 | pconst _ c q => well_c c /\ well_p q
 end.
 
-Lemma seq_hoare_triple :
-forall c l p la ps P Q R,
-hoare_triple_c P R c l la ps ->
-hoare_triple_p (fun l => R (Post |-> l Pre ; (Pre |-> la Pre ; l) )) Q p la ps ->
-hoare_triple_p P Q (pconst l c p) la ps.
-Proof.
-intros.
-unfold hoare_triple_p.
-unfold ceval_f_i_p.
-intros.
-unfold hoare_triple_c in H.
-unfold ceval_f_i_c in H.
-unfold hoare_triple_p in H0.
-unfold ceval_f_i_p in H0.
-destruct i.
-+ simpl. auto.
-+ simpl. 
-Abort.
- 
-
 Lemma correct :
-forall p la ps,
+forall p ps pi,
 well_p p ->
-forall (P Q: lambda -> Prop),
-(forall la m m', P (Pre |-> m ; la ) -> tp p la m (fun m _ => m = m') ps -> Q (Post |-> m' ; (Pre |-> m ; la ))) -> 
-hoare_triple_p P Q p la ps.
+forall (P Q: assertion),
+(forall m la, P m la -> tp p la m pi (fun m' la' => Q m' la')) -> 
+hoare_triple_p P Q p ps.
 Proof.
-intros p la ps.
+intros p ps pi.
 elim p using prog_com_ind with 
   (P :=  fun c : com =>
   well_c c ->
-  forall la l (P Q: lambda -> Prop),
-  (forall la m m', P (Pre |-> m ; la ) -> tc c l la m m' ps -> Q (Post |-> m' ; (Pre |-> m ; la ))) -> 
-    hoare_triple_c P Q c l la ps).
-* intros. unfold hoare_triple_c. intros.  unfold ceval_f_i_c. destruct i. 
-  + simpl. auto.
-  + simpl. simpl in H0. apply H0. assumption. reflexivity.
-* intros. unfold hoare_triple_c. intros.  unfold ceval_f_i_c. destruct i.
-  + simpl. auto.
-  + contradiction H.
-* intros. unfold hoare_triple_c. intros.  unfold ceval_f_i_c. destruct i.
-  + simpl. auto.
-  + contradiction H.
-* intros. unfold hoare_triple_c. intros.  unfold ceval_f_i_c. destruct i.
-  + simpl. auto.
-  + contradiction H1.
-* intros. unfold hoare_triple_c. intros.  unfold ceval_f_i_c. destruct i.
-  + simpl. auto.
-  + contradiction H0.
-* intros. unfold hoare_triple_c. intros.  unfold ceval_f_i_c. destruct i.
-  + simpl. auto.
-  + contradiction H.
-* intros. unfold hoare_triple_p. intros.  unfold ceval_f_i_p. destruct i.
-  + simpl. auto.
-  + simpl. apply H0. assumption.  reflexivity.
-*  intros. apply seq_hoare_triple.
+  forall l (P Q: assertion),
+  (forall la m m', P m la ->  tc c l la m m' pi (Q  m' (l |-> m ; la ))) -> 
+    hoare_triple_c P Q c l ps).
+* intros. unfold hoare_triple_c. intros. apply (H0 la s s').
+  + assumption.
+  + inversion H2;subst. reflexivity.
+* intros. unfold hoare_triple_c. intros. apply (H0 la s s').
+  + assumption.
+  + inversion H2;subst. 
+    unfold set.
+ 
+    unfold update_sigma.
+    (* reflexivity. *) contradiction H.
+* intros.  contradiction H.
+* intros. contradiction H1. (*apply if_hoare_triple.*)
+  
+* intros. contradiction H0.
+* intros. unfold hoare_triple_p. intros. eapply H0. inversion H2;subst. assumption.
+* intros.
+  apply (seq_hoare_triple _ _ _ _ _ _ 
+    (fun m la => tp p0 la m pi (fun (m'0 : sigma) (la' : lambda) => Q m'0 la'))).
+  +  apply H.
+    - simpl in H1. destruct H1. assumption.
+    - intros. simpl in H2. apply H2. assumption. 
+  + apply H0. 
+    - simpl in H1. destruct H1. assumption.
+    - eauto.
+Qed.
 
+Lemma seq_vc :
+forall c l p ps (P Q R: lambda -> Prop),
+forall la m m' m'',  
+((P (Pre |-> m ; la ) -> tc c l la m m'' ps -> R (Post |-> m'' ; (Pre |-> m ; (l |-> m ; la ) ))) /\ 
+(R (Post |-> m'' ; (Pre |-> m ; (l |-> m ; la ) )) -> tp p (l |-> m ; la ) m'' (fun (m0 : sigma) (_ : lambda) => m0 = m') ps -> Q (Post |-> m' ; (Pre |-> m ; la )))) ->
+(P (Pre |-> m; la) -> tp (pconst l c p) la m (fun (m0 : sigma) (_ : lambda) => m0 = m') ps -> Q (Post |-> m'; Pre |-> m; la)).
+Proof.
+intros c l p ps P Q R la m m' m'' H Pre H12.
+simpl in H12.
+specialize (H12 m'').
+destruct H12.
+destruct H.
+apply H2.
+apply H.
+all: try assumption.
+Abort.
+
+  
