EVcg.v
@@ -1,104 +1,263 @@
 From Coq Require Import PeanoNat.
 From Rela Require Import Aexp.
 From Rela Require Import Bexp.
-From Rela Require Import EAexp.
-From Rela Require Import EBexp.
 From Rela Require Import ECom.
 From Rela Require Import Proc.
 From Rela Require Import Label.
 From Rela Require Import Lambda.
+From Rela Require Import Sigma.
+From Rela Require Import Loc.
 
 From Coq Require Import Bool.Bool.
 From Coq Require Import Init.Nat.
 From Coq Require Import Arith.Arith.
 From Coq Require Import Arith.EqNat.
 
-(* Why3 goal *)
-Definition set: (nat -> nat) -> nat -> nat -> nat -> nat.
+From Coq Require Import Lia.
+
+Definition set: (Loc.t -> nat) -> Loc.t -> nat -> Loc.t -> nat.
 Proof.
 intros m x y.
 intros x'.
-Locate Nat.eq_dec .
-destruct (Nat.eq_dec x x') as [H|H].
+destruct (Loc.eq_dec x x') as [H|H].
 exact y.
 exact (m x').
 Defined.
 
 Lemma set'def:
-  forall (f: nat -> nat ) (x:nat) (v:nat) (y:nat),
+  forall (f: Loc.t -> nat ) (x: Loc.t) (v:nat) (y: Loc.t),
   ((y = x) -> ((set f x v y) = v)) /\ (~ (y = x) -> ((set f x v y) = (f y))).
 Proof.
 intros f x v y.
 split.
 + intros.
  unfold set.
- destruct (Nat.eq_dec x y).
+ destruct (Loc.eq_dec x y).
   * reflexivity.
   * contradiction n.
     rewrite H. reflexivity.
 + intros. 
   unfold set.
- destruct (Nat.eq_dec x y).
+ destruct (Loc.eq_dec x y).
   * contradiction H.
     rewrite e. reflexivity.
   * reflexivity.
 Qed.
 
+(** Definition of Precondtion **)
+
+Definition precondition : Type := sigma -> Prop.
+
+Definition empty_precondition : precondition := (fun _ => True).
+
+(** Defintion of Postcondtion **)
+
+Definition postcondition : Type := sigma -> sigma -> Prop.
+
+Definition empty_postcondition :  postcondition := (fun _ _ => True).
+
+(** Definition of a contract **)
+
+Definition clause : Type := precondition * postcondition.
+
+Definition empty_clause : clause := (empty_precondition, empty_postcondition). 
+
+Module Phi.
+
+  (** The programs that can be called is a maps from procedure to program **)
+
+  Definition phi : Type := Proc.t -> clause.
+
+  Definition update_psi (x:Proc.t) (v: clause) (l:phi): phi :=
+  fun (x': Label.t) => if Proc.eqb x' x then v else l x'.
+
+  Notation "x '#->' v ; l" := (update_psi x v l)(at level 100, v at next level, right associativity).
+
+  Definition get_pre (an:clause) := 
+          let (pre,post) := an in
+          pre.
+
+  Definition get_post (an:clause) := 
+          let (pre,post) := an in
+          post.
+
+End Phi.
+
+Inductive branch (A B C : Prop) : Prop :=  
+  | Then : A -> B -> branch A B C
+  | Else : ~ A -> C -> branch A B C.
+
 Fixpoint tc (c : com) (l: Label.t) (s : Lambda.lambda) (m m' : Sigma.sigma)
-            (ps: Psi.psi): Prop :=
+            (ps: Phi.phi) (suite : Prop) : Prop :=
     match c with
-    | CSkip => m = m'
-    | CAss x a => m' = (set m x (aeval m a))
-    | CAssert b => ebeval_prop (l |-> m; s) b /\ m = m'
+    | CSkip => m = m' -> suite
+    | CAss x a => (m' = set m x (aeval m a)) -> suite
+    | CAssert b => b m s -> m = m' -> suite
     | CIf b p1 p2 =>
-        beval m b = true -> tp p1 (l |-> m; s) m (fun m _ => m = m') ps /\
-        beval m b = false -> tp p2 (l |-> m; s) m (fun m _ => m = m') ps
-    | CWhile b c inv ass =>  
-            ebeval_prop (Here |-> m; s) inv /\
-            ebeval_prop (Here |-> m; s) inv /\
-            beval m' b = false
-    | CCall proc => 
-          let s' := (Pre |-> m; s) in 
-          let (_,annot) := ps proc in
-          ebeval_prop s' (Psi.get_pre annot) /\
-          ebeval_prop (Post |-> m'; s') (Psi.get_post annot)
+         forall m1, tp p1 (l |-> m1; s) m1 ps (fun m1' _ => 
+             forall m2, tp p2 (l |-> m2;s) m2 ps (fun m2' _ => 
+               (branch (beval m b = true) (m' = m1' /\ m = m1) (m' = m2' /\ m = m2) -> suite) 
+            )
+         )
+    | CWhile b p inv _ => inv m (l |->m; s) -> inv m' (l |->m; s) -> beval m b = false -> suite 
     end
-  with tp (p : prog) (s : Lambda.lambda) (m: Sigma.sigma)
-            (fin: Sigma.sigma -> Lambda.lambda -> Prop)
-            (ps: Psi.psi): Prop :=
+ with tp (p : prog) (s : Lambda.lambda) (m: Sigma.sigma)  (ps: Phi.phi)
+            (fin: Sigma.sigma -> Lambda.lambda -> Prop)  : Prop :=
+  match p with
+  | pnil => fin m s
+  | pconst l c p' => forall m', tc c l s m m' ps (tp p' (l |-> m; s) m' ps fin)
+end.
+
+Definition empty_phi: Phi.phi := fun _ => empty_clause.
+
+Lemma test1 : forall s m,  m EAX = 1 -> tp plus2 s m empty_phi (fun m' s' => m' EAX = 3) .
+Proof.
+simpl.
+intros.
+Abort.
+
+Definition plus3 : prog := pconst l1 (CAss EAX (APlus (AId EAX) (ANum 2)))
+                          (pconst l2 (CAss EAX (APlus (AId EAX) (ANum 2))) pnil).
+
+Lemma test2 : forall s m, m EAX = 1 -> tp plus3 s m empty_phi (fun m' s' => m' EAX = 5).
+Proof.
+  simpl.
+  intros.
+Abort.
+
+Definition if2 : prog := pconst l1 (CIf (BEq (AId EAX) (ANum 4)) plus2 plus2 ) pnil.
+
+Lemma test3 : forall s m, m EAX = 1 -> tp if2 s m empty_phi ( fun m' s' => m' EAX = 3).
+Proof.
+  simpl.
+  intros.
+Abort.
+
+Definition if3 : prog := pconst l1 (CAss EAX (APlus (AId EAX) (ANum 2)))
+                         (pconst l1 (CIf (BEq (AId EAX) (ANum 4)) plus2 plus2) plus2).
+
+Lemma test4 : forall s m, m EAX = 1 -> tp if3 s m empty_phi ( fun m' s' => m' EAX = 3).
+Proof.
+  simpl.
+  intros.
+Abort.
+
+Lemma test5 : forall s m1 m2, m1 EAX = m2 EAX -> 
+                              tp plus2 s m1 empty_phi ( fun m1' _ => 
+                              tp plus2 s m2 empty_phi ( fun m2' _ =>
+                                     m1' EAX = m2' EAX)).
+Proof.
+  simpl.
+  intros.
+Abort.
+
+Fixpoint tc' (c : com) (l: Label.t) (s : Lambda.lambda) (m m' : Sigma.sigma)
+            (ps: Phi.phi) (suite : Prop) : Prop :=
+    match c with
+    | CSkip => tc c l s m m' ps suite
+    | CAss x a => tc c l s m m' ps suite
+    | CAssert b => b m s /\ tc c l s m m' ps suite
+    | CIf b p1 p2 => 
+         (beval m b = true -> tp' p1 (l |->m; s) m ps) /\
+         (beval m b = false -> tp' p2 (l |->m; s) m ps) /\
+          tc c l s m m' ps suite
+    | CWhile b p inv _ => 
+      (beval m b = true -> inv m (l |->m; s)) /\ 
+      (beval m b = true -> forall mi, inv mi (l |->m; s) -> 
+                           tp p (l |->m; s) m ps (fun sf mf => inv sf mf)) /\ 
+      (beval m b = true -> forall mi, inv mi (l |->m; s) -> tp' p (l |->m; s) m ps) /\ 
+      tc c l s m m' ps suite
+    end
+ with tp' (p : prog) (s : Lambda.lambda) (m: Sigma.sigma)  (ps: Phi.phi) : Prop :=
+  match p with
+  | pnil => True
+  | pconst l c p' => forall m', tc' c l s m m' ps (tp' p' (l |-> m; s) m' ps)
+end.
+
+Definition truc3 : prog := pconst l1 (CAssert (fun m _ => m EAX = 2))
+                          (pconst l2 (CAssert (fun m _ => m EAX = 2)) pnil).
+                          
+Lemma test4 : forall s m, (m EAX = 2) -> tp' truc3 s m  empty_phi .
+Proof.
+intros.
+simpl.
+intros.
+split. 
+  * assumption.
+  * intros. split.
+    - rewrite <- H1. assumption.
+    - intros. auto. 
+Qed.
+
+Definition if4 : prog := pconst l1 (CIf (BEq (AId EAX) (ANum 2)) (pconst l1 (CAssert (fun m _ => m EAX = 2)) pnil) pnil) pnil.
+
+Lemma test5 : forall s m, (m EAX = 2) -> tp' if4 s m  empty_phi .
+Proof.
+intros.
+simpl.
+intros.
+split. 
+  * intros. split. all: try auto.
+  * split.
+    - auto.
+    - intros. auto. 
+Qed.
+ 
+(*Fixpoint tc' (c : com) (l: Label.t) (s : Lambda.lambda) (m m' : Sigma.sigma)
+            (suite : Prop -> Prop-> Prop) (fin : Prop) (vc : Prop)
+            (ps: Phi.phi): Prop :=
+    match c with
+    | CSkip => suite vc (m = m')
+    | CAss x a => suite vc (m' = set m x (aeval m a))
+    | CAssert b => suite (vc /\ (fin -> b m s)) (m = m' /\ b m s)
+    | _ => suite vc (True)
+    end
+ with tp' (p : prog) (s : Lambda.lambda) (m: Sigma.sigma)
+            (fin: Prop) (vc :Prop)
+            (ps: Phi.phi) : Prop :=
+  match p with
+  | pnil => vc
+  | pconst l c p' => 
+       forall m', tc' c l s m m' (fun (vcs : Prop) (vc : Prop) => 
+                     tp' p' (l |-> m; s) m' (vc -> fin) vcs ps ) fin vc ps
+end.*)
+
+
+
+(**************************************************************)
+(*                      TRASH                                 *)
+(**************************************************************)
+
+
+(*
+
+Fixpoint tc (c : com) (l: Label.t) (s : Lambda.lambda) (m m' : Sigma.sigma)
+            (ps: Phi.phi) (suite : Prop -> Prop) : Prop :=
+    match c with
+    | CSkip => suite (m = m')
+    | CAss x a => suite (m' = set m x (aeval m a))
+    | CAssert b => suite (m = m' /\ b m s)
+    | CIf b p1 p2 =>
+         tp p1 s m ps (fun m1 _ => 
+             tp p2 s m ps (fun m2 _ => 
+               suite (branch (beval m b = true) (m' = m1) (m' = m2)) 
+            )
+         )
+    | _ => suite (True)
+    end
+ with tp (p : prog) (s : Lambda.lambda) (m: Sigma.sigma)  (ps: Phi.phi)
+            (fin: Sigma.sigma -> Lambda.lambda -> Prop)  : Prop :=
   match p with
   | pnil => fin m s
   | pconst l c p' => 
-    forall m' : Sigma.sigma, tc c l s m m' ps -> tp p' (l |-> m; s) m' fin ps
+       forall m', tc c l s m m' ps (fun (vc : Prop)  => 
+                      tp p' (l |-> m; s) m' ps (fun mf sf => vc -> fin mf sf)
+                  )
 end.
 
+*)
 
-(*Fixpoint vc_aux (c : prog') (acc : prog') (s : nat -> (nat -> nat)) (m: nat -> nat)
-                (annot: Proc.t ->  clause): Prop := 
- match c with
-    | pnil => True
-    | pconst (CSkip' l) p => 
-      vc_aux p (append (CSkip' l) acc) s m annot
-    | pconst (CAss' l x a) p =>
-      vc_aux p (append (CAss' l x a) acc) s m annot
-    | pconst (CAssert' l b) p =>
-      tc acc m s (fun _ s => teb s b) annot /\ vc_aux p (append (CAssert' l b) acc) s m annot
-    | pconst (CIf' l b p1 p2) p =>
-      tc acc m s (fun s m => tb b m = true -> vc_aux p1 pnil s m annot) annot /\
-      tc acc m s (fun s m => tb b m = false -> vc_aux p2 pnil s m annot) annot /\
-      vc_aux p (append (CIf' l b p1 p2) acc) s m annot
-    | pconst (CWhile' l b c inv ass) p => 
-      tc acc m s (fun s m => teb (fun l' => if Label.Label.eqb l' Label.Here then m else s l') inv ) annot /\
- 
-     (* the historic in not required because we have don't use assigns (for the momment) *)
-      (forall m : nat -> nat, forall s: nat -> (nat -> nat),
-      teb (fun l' => if Label.Label.eqb l' Label.Here then m else s l') inv ->
-      tc p m s (fun s m => teb (fun l' => if Label.Label.eqb l' Label.Here then m else s l') inv ) annot
-      )
-      vc_aux p (append (CWhile' l b c inv ass) acc) s m annot
-    | pconst (CCall' l proc) p => 
-      vc_aux p (append (CCall' l proc) acc) s m annot
-end.*)
+
 
 (*Definition vc_f (ps: Psi.psi): Prop :=
 forall (f :Proc.t) la m m', 
@@ -107,5 +266,86 @@ forall (f :Proc.t) la m m',
   (Psi.get_post (Psi.get_an f ps)) (Post |-> m' ; (Pre |-> m ; la )).*)
 
 
+
+
+(*
+
+Fixpoint tc (c : com) (l: Label.t) (s : Lambda.lambda) (m m' : Sigma.sigma)
+            (ps: Phi.phi): Prop :=
+    match c with
+    | CSkip => m = m'
+    | CAss x a => m' = (set m x (aeval m a))
+    | CAssert b => b m s /\ m = m'
+    | _ => False
+    end
+  with tp (p : prog) (s : Lambda.lambda) (m: Sigma.sigma)
+            (fin: Sigma.sigma -> Lambda.lambda -> Prop)
+            (ps: Phi.phi) : Prop :=
+  match p with
+  | pnil => fin m s
+  | pconst l c p' => 
+    forall m' : Sigma.sigma, 
+        tp p' (l |-> m; s) m' (fun mf sf => tc c l s m m' ps -> fin mf sf) ps 
+end.
+
+Lemma correct :
+forall p ps pi m la m' la' i,
+well_p p ->
+tp p la m (fun m la => m = m' /\ la = la') pi ->
+ceval_step_prog m la ps p i = Some(m', la') \/ 
+ceval_step_prog m la ps p i = None.
+Proof.
+intros p ps pi m la m' la' i Well.
+generalize dependent m.
+generalize dependent la.
+generalize dependent m'.
+generalize dependent la'.
+generalize dependent Well.
+elim p using prog_com_ind with 
+  (P :=  fun c : com =>
+   well_c c ->
+   forall m m' la l,
+      tc c l la m m' pi ->
+      ceval_step_com m l la ps c i  = Some (m', (l |-> m ; la )) \/
+      ceval_step_com m l la ps c i  = None).
+    * intros. destruct (ceval_step_com m l la ps CSkip i) eqn:Heqr.
+      - left. destruct p0.
+        destruct i.
+        + discriminate Heqr.
+        + simpl in H0. simpl in Heqr. inversion Heqr;subst. reflexivity.
+      - right. reflexivity.
+    * intros. contradiction H.
+    * intros. contradiction H.
+    * intros. contradiction H1.
+    * intros. contradiction H0.
+    * intros. destruct (ceval_step_prog m la ps pnil i) eqn:Heqr.
+      - left. destruct p0.
+        destruct i.
+        + discriminate Heqr.
+        + simpl in H. simpl in Heqr. destruct H. inversion Heqr;subst. reflexivity.
+      - right. reflexivity. 
+    * intros.
+      destruct (ceval_step_prog m la ps (pconst t c p0) i) eqn: Heqr1.
+        - left. destruct p1.
+          destruct i.
+          + discriminate Heqr1.
+          + simpl in Heqr1.
+          destruct (ceval_step_com m t la ps c i) eqn: Heqr2.
+            ** destruct i.
+              -- discriminate Heqr2.
+              -- destruct p1.
+                 simpl in H1.
+                 specialize (H1 s0).
+                 destruct H1.
+                 apply H0 in H2. destruct H2.
+                 apply H in H1. destruct H1.
+                 apply (ceval_step_more (S i) ( S (S i))) in Heqr1.
+                 rewrite H2 in Heqr1.
+                 inversion Heqr1;subst.
+                 reflexivity.
+                 lia.
+                 simpl in Well.
+
+Qed.*)
 
 (*define function for proving assertion and invariant: generate sub program by visiting program*)
